theories/Analysis/ContextMap.v
@@ -1,0 +1,433 @@
+Require Import Max Nat CMap Infra.Lattice Infra.PartialOrder CMapPartialOrder.
+
+Set Implicit Arguments.
+
+Record ctxmap X := {
+                     ctxmap_M : Map [nat, X];
+                     ctxmap_len : nat
+                   }.
+
+Definition ctxmap_to_idx X (m:ctxmap X) (n:nat) :=
+  ctxmap_len m - S n.
+
+Definition ctxmap_emp X : ctxmap X :=
+  Build_ctxmap (@MapInterface.empty nat _ _ X) 0.
+
+Definition ctxmap_update_at X (m:ctxmap X) (n:nat) (x:X)
+  := if [n >= ctxmap_len m] then m
+    else Build_ctxmap (add (ctxmap_to_idx m n) x (ctxmap_M m)) (ctxmap_len m).
+
+Definition ctxmap_join_at X `{JoinSemiLattice X} (m:ctxmap X) (n:nat) (x:X)
+  := let k := ctxmap_to_idx m n in
+    let v := match MapInterface.find k (ctxmap_M m) with
+            | Some y => join x y
+            | None => x
+            end in
+    Build_ctxmap (add k v (ctxmap_M m)) (ctxmap_len m).
+
+Fixpoint range (n d:nat) :=
+  match d with
+  | 0 => nil
+  | S d => n::range (S n) d
+  end.
+
+Definition ctxmap_app X (m:ctxmap X) (L:list X)
+  := let l := length L in
+    Build_ctxmap ((ctxmap_M m)[-range (ctxmap_len m) l <-- L -]) (ctxmap_len m + l).
+
+Fixpoint ctxmap_erase X (m:Map [nat, X]) Z : Map [nat, X]
+  := match Z with
+    | nil => m
+    | x::Z => MapInterface.remove x (@ctxmap_erase X m Z)
+    end.
+
+Definition ctxmap_extend X (m:ctxmap X) (n:nat) :=
+  Build_ctxmap (ctxmap_erase (ctxmap_M m) (range (ctxmap_len m) n))
+               (ctxmap_len m + n).
+
+
+Definition ctxmap_at X m n : option X
+  := if [n >= ctxmap_len m] then None
+    else MapInterface.find (ctxmap_to_idx m n) (ctxmap_M m).
+
+Lemma ctxmap_at_gt X m x
+  : x >= ctxmap_len m ->  @ctxmap_at X m x = None.
+Proof.
+  unfold ctxmap_at. intros; cases. reflexivity.
+Qed.
+
+Definition ctxmap_drop (n:nat) X (m:ctxmap X)  :=
+  Build_ctxmap (ctxmap_M m) (ctxmap_len m - n).
+
+Definition ctxmap_poLe X `{PartialOrder X} (m m':ctxmap X) :=
+  ctxmap_len m = ctxmap_len m'
+  /\ forall x, x < ctxmap_len m -> poLe (MapInterface.find x (ctxmap_M m))
+                                 (MapInterface.find x (ctxmap_M m')).
+
+Definition ctxmap_poEq X `{PartialOrder X} (m m':ctxmap X) :=
+  ctxmap_len m = ctxmap_len m'
+  /\ forall x, x < ctxmap_len m -> poEq (MapInterface.find x (ctxmap_M m))
+                                 (MapInterface.find x (ctxmap_M m')).
+
+Fixpoint nat_quant_dec P `{H:forall x, Computable (P x) } k : bool  :=
+  match k with
+  | 0 => true
+  | S k => if [P k] then nat_quant_dec P k else false
+  end.
+
+
+Instance nat_quant_computable k P
+         `{forall x, Computable (P x) } :
+  Computable (forall x, x < k -> P x).
+Proof.
+  hnf. remember (nat_quant_dec P k).
+  induction k;
+    simpl in *; repeat cases in Heqb; clear_trivial_eqs.
+  - left. intros. inv H0.
+  - edestruct IHk; eauto.
+    + left. intros. inv H0; eauto.
+    + right. intro. eapply n; intros. eapply H0. omega.
+  - right. intro. eapply NOTCOND. eapply H0. eauto.
+Qed.
+
+Instance ctxmap_poLe_dec X `{PartialOrder X} m m'
+  : Computable (ctxmap_poLe m m').
+Proof.
+  hnf. decide (ctxmap_len m = ctxmap_len m');[|right; inversion 1; eauto].
+  unfold ctxmap_poLe.
+  enough ({(forall x : nat, x < ctxmap_len m ->
+                     MapInterface.find x (ctxmap_M m)
+                                       ⊑ MapInterface.find x (ctxmap_M m'))} +
+          {~ (forall x : nat, x < ctxmap_len m ->
+                       MapInterface.find x (ctxmap_M m)
+                                         ⊑ MapInterface.find x (ctxmap_M m'))}). {
+    destruct H0; eauto.
+  }
+  eapply nat_quant_computable.
+  intros. eapply poLe_dec.
+Qed.
+
+Instance ctxmap_poEq_dec X `{PartialOrder X} m m'
+  : Computable (ctxmap_poEq m m').
+Proof.
+  hnf. decide (ctxmap_len m = ctxmap_len m');[|right; inversion 1; eauto].
+  unfold ctxmap_poLe.
+  enough ({(forall x : nat, x < ctxmap_len m ->
+                     MapInterface.find x (ctxmap_M m)
+                                       ≣ MapInterface.find x (ctxmap_M m'))} +
+          {~ (forall x : nat, x < ctxmap_len m ->
+                       MapInterface.find x (ctxmap_M m)
+                                         ≣ MapInterface.find x (ctxmap_M m'))}). {
+    destruct H0; eauto 20.
+    left. split. eauto. eauto.
+    right. inversion 1. eauto.
+  }
+  eapply nat_quant_computable.
+  intros. eapply poEq_dec.
+Qed.
+
+Instance ctxmap_poEq_refl X `{PartialOrder X}
+  : Reflexive (ctxmap_poEq (X:=X)).
+Proof.
+  hnf; intros; unfold ctxmap_poEq; intros.
+  eauto.
+Qed.
+
+Instance ctxmap_poEq_sym X `{PartialOrder X}
+  : Symmetric (ctxmap_poEq (X:=X)).
+Proof.
+  hnf; intros; unfold ctxmap_poEq; intros.
+  exploit H0; dcr. rewrite H2 in *. split; eauto.
+  intros. rewrite H3; eauto.
+Qed.
+
+Instance ctxmap_poEq_trans X `{PartialOrder X}
+  : Transitive (ctxmap_poEq (X:=X)).
+Proof.
+  unfold ctxmap_poEq.
+  hnf; intros; dcr. split; intros; eauto.
+  - congruence.
+  - rewrite H4; eauto. rewrite H3; eauto. omega.
+Qed.
+
+
+Instance ctxmap_poLe_trans X `{PartialOrder X}
+  : Transitive (ctxmap_poLe(X:=X)).
+Proof.
+  unfold ctxmap_poLe.
+  hnf; intros; dcr. split; intros; eauto.
+  - congruence.
+  - rewrite H4; eauto. rewrite H3; eauto. omega.
+Qed.
+
+Instance ctxmap_poEq_Equivalene X `{PartialOrder X}
+  :  Equivalence (ctxmap_poEq (X:=X)).
+Proof.
+  econstructor; eauto with typeclass_instances.
+Defined.
+
+Instance ctxmap_poLe_anti X `{PartialOrder X}
+  : Antisymmetric (ctxmap X) (ctxmap_poEq (X:=X)) (ctxmap_poLe (X:=X)).
+Proof.
+  unfold ctxmap_poEq, ctxmap_poLe.
+  hnf; intros; dcr. split.
+  - congruence.
+  - intros. rewrite H2 in *.
+    eapply antisymmetry; eauto.
+Qed.
+
+Instance ctxmap_po X `{PartialOrder X} : PartialOrder (ctxmap X) :=
+  {
+    poLe := @ctxmap_poLe X _;
+    poEq := @ctxmap_poEq X _
+  }.
+Proof.
+  unfold ctxmap_poLe. intros.
+  - destruct H0. split; eauto.
+Defined.
+
+
+Lemma ctxmap_at_poLe X `{PartialOrder X} m m' x
+  : m ⊑ m'
+    -> ctxmap_at m x ⊑ ctxmap_at m' x.
+Proof.
+  intros. destruct H0.
+  unfold ctxmap_at; repeat cases; try rewrite H0; eauto;
+    try now (exfalso; omega).
+  unfold ctxmap_to_idx. rewrite H0.
+  eapply H1. omega.
+Qed.
+
+Lemma ctxmap_at_poEq X `{PartialOrder X} m m' x
+  : m ≣ m'
+    -> ctxmap_at m x ≣ ctxmap_at m' x.
+Proof.
+  intros. destruct H0.
+  unfold ctxmap_at; repeat cases; try rewrite H0; eauto;
+    try now (exfalso; omega).
+  unfold ctxmap_to_idx. rewrite H0.
+  eapply H1; eauto. omega.
+Qed.
+
+Hint Resolve ctxmap_at_poLe ctxmap_at_poEq.
+
+Lemma ctxmap_update_at_poLe X `{PartialOrder X} m m' v v' x
+  : m ⊑ m'
+    -> v ⊑ v'
+    -> ctxmap_update_at m x v ⊑ ctxmap_update_at m' x v'.
+Proof.
+  intros.
+  unfold poLe; simpl. destruct H0.
+  unfold ctxmap_update_at, ctxmap_poLe, ctxmap_at, ctxmap_to_idx; simpl.
+  repeat cases; eauto; intros; repeat cases; eauto; simpl in *;
+    try now (exfalso; omega).
+  split; eauto.
+  intros; eauto.
+  decide (x = x0); subst.
+  + mlud; eauto. exfalso. rewrite H0 in *. eauto.
+    exfalso. rewrite H0 in *. eauto.
+  + mlud; eauto.
+    exfalso. rewrite H0 in *; eauto.
+    exfalso. rewrite H0 in *; eauto.
+Qed.
+
+Hint Resolve ctxmap_update_at_poLe.
+
+Lemma ctxmap_update_at_poEq X `{PartialOrder X} m m' v v' x
+  : m ≣ m'
+    -> v ≣ v'
+    -> ctxmap_update_at m x v ≣ ctxmap_update_at m' x v'.
+Proof.
+  intros.
+  unfold poEq; simpl. destruct H0.
+  unfold ctxmap_update_at, ctxmap_poEq, ctxmap_at, ctxmap_to_idx; simpl.
+  repeat cases; eauto; intros; repeat cases; eauto; simpl in *;
+    try now (exfalso; omega).
+  split; eauto.
+  intros; repeat cases; eauto; try now (exfalso; omega).
+  decide (x = x0); subst.
+  + mlud; eauto. econstructor. eauto.
+    exfalso. rewrite H0 in *. eauto.
+    exfalso. rewrite H0 in *. eauto.
+  + mlud; eauto. econstructor; eauto.
+    exfalso; rewrite H0 in *; eauto.
+    exfalso; rewrite H0 in *; eauto.
+Qed.
+
+Hint Resolve ctxmap_update_at_poEq.
+
+
+Lemma ctxmap_join_at_poLe X `{JoinSemiLattice X} (m m':ctxmap X) v v' x
+  : m ⊑ m'
+    -> v ⊑ v'
+    -> ctxmap_join_at m x v ⊑ ctxmap_join_at m' x v'.
+Proof.
+  intros.
+  unfold poLe; simpl. destruct H1.
+  unfold ctxmap_join_at, ctxmap_poLe, ctxmap_at, ctxmap_to_idx; simpl.
+  split; eauto.
+  intros.
+  mlud; eauto.
+  + exploit (H3 (ctxmap_len m - S x)). omega.
+    rewrite <- H1 in *.
+    revert H5; repeat cases; simpl; intros; clear_trivial_eqs; eauto.
+    econstructor. rewrite H5, H2. reflexivity.
+    econstructor. rewrite H2. eapply join_poLe.
+  + exfalso. rewrite H1 in *. eauto.
+  + exfalso. rewrite H1 in *. eauto.
+Qed.
+
+Lemma ctxmap_join_at_poEq X `{JoinSemiLattice X} m m' v v' x
+  : m ≣ m'
+    -> v ≣ v'
+    -> ctxmap_join_at m x v ≣ ctxmap_join_at m' x v'.
+Proof.
+  intros.
+  unfold poEq; simpl. destruct H1.
+  unfold ctxmap_join_at, ctxmap_poEq, ctxmap_at, ctxmap_to_idx; simpl.
+  split; eauto.
+  intros.
+  mlud; eauto.
+  + exploit (H3 (ctxmap_len m - S x)). omega.
+    rewrite <- H1 in *.
+    revert H5; repeat cases; simpl; intros; clear_trivial_eqs; eauto.
+    econstructor. rewrite H5, H2. reflexivity.
+    econstructor. rewrite H2. eauto.
+  + exfalso. rewrite H1 in *. eauto.
+  + exfalso. rewrite H1 in *. eauto.
+Qed.
+
+Hint Resolve ctxmap_join_at_poLe ctxmap_join_at_poEq.
+
+
+Lemma ctxmap_drop_poLe X `{PartialOrder X} n m m'
+  : m ⊑ m'
+    -> ctxmap_drop n m ⊑ ctxmap_drop n m'.
+Proof.
+  intros. destruct H0.
+  unfold ctxmap_drop; hnf. simpl.
+  split; eauto. intros. eapply H1. omega.
+Qed.
+
+Lemma ctxmap_drop_poEq X `{PartialOrder X} n m m'
+  : m ≣ m'
+    -> ctxmap_drop n m ≣ ctxmap_drop n m'.
+Proof.
+  intros. destruct H0.
+  unfold ctxmap_drop; hnf. simpl.
+  split; eauto. intros.
+  eapply H1; eauto. omega.
+Qed.
+
+Hint Resolve ctxmap_drop_poLe ctxmap_drop_poEq.
+
+Lemma ctxmap_erase_poLe_single X `{PartialOrder X} n m m' x
+  : MapInterface.find x m ⊑ MapInterface.find x m'
+    -> MapInterface.find x (ctxmap_erase m n)
+                        ⊑ MapInterface.find x (ctxmap_erase m' n).
+Proof.
+  intros. general induction n; simpl; eauto.
+  mlud; eauto.
+Qed.
+
+Lemma ctxmap_erase_poEq_single X `{PartialOrder X} n m m' x
+  : MapInterface.find x m ≣ MapInterface.find x m'
+    -> MapInterface.find x (ctxmap_erase m n)
+                        ≣ MapInterface.find x (ctxmap_erase m' n).
+Proof.
+  intros. general induction n; simpl; eauto.
+  mlud; eauto.
+Qed.
+
+Lemma ctxmap_erase_poLe X `{PartialOrder X} n m m'
+  : m ⊑ m'
+    -> ctxmap_erase m n ⊑ ctxmap_erase m' n.
+Proof.
+  intros. general induction n; simpl; eauto.
+  eapply leMap_remove. eapply IHn. eauto.
+Qed.
+
+Instance remove_poEq X `{PartialOrder X} (x:nat)
+  : Proper (poEq ==> poEq) (MapInterface.remove x).
+Proof.
+  unfold Proper, respectful; intros.
+  hnf; intros. mlud; eauto.
+Qed.
+
+Lemma remove_remove X `{PartialOrder X} m (a b:nat)
+  : MapInterface.remove a (MapInterface.remove b m)
+                        ≣ MapInterface.remove b (MapInterface.remove a m).
+Proof.
+  hnf; intros.
+  repeat mlud; eauto.
+Qed.
+
+Lemma remove_erase X `{PartialOrder X} m Z a
+  : MapInterface.remove a (ctxmap_erase m Z) ≣ (ctxmap_erase (MapInterface.remove a m) Z).
+Proof.
+  general induction Z; simpl; eauto.
+  rewrite remove_remove. rewrite IHZ. reflexivity.
+Qed.
+
+Lemma ctxmap_erase_poEq X `{PartialOrder X} Z m m' x
+  : x ∈ of_list Z
+    -> MapInterface.find x (ctxmap_erase m Z)
+                        ≣  MapInterface.find x (ctxmap_erase m' Z).
+Proof.
+  intros. general induction Z; simpl in *; eauto.
+  - simpl in *. cset_tac.
+  - cset_tac'.
+    + mlud; eauto. exfalso; eauto.
+    + rewrite !remove_erase. eapply IHZ. eauto.
+Qed.
+
+
+Lemma x_notin_range x k n
+  : x ∉ of_list (range k n)
+    -> x < k \/ k+n <= x.
+Proof.
+  general induction n; simpl in *.
+  - decide (x < k); omega.
+  - decide (x = k); subst;
+      cset_tac'. eapply IHn in H1. destruct H1.
+    omega. omega.
+Qed.
+
+Lemma x_in_range x k n
+  : x >= k /\ k+n > x -> x ∈ of_list (range k n).
+Proof.
+  general induction n; simpl in *; dcr.
+  - exfalso; omega.
+  - decide (x = k); subst;
+      cset_tac'. eapply IHn. omega.
+Qed.
+
+Lemma ctxmap_extend_poLe X `{PartialOrder X} n m m'
+  : m ⊑ m'
+    -> ctxmap_extend m n ⊑ ctxmap_extend m' n.
+Proof.
+  intros. destruct H0.
+  unfold ctxmap_extend; hnf. simpl.
+  split; eauto. intros.
+  decide (x < ctxmap_len m).
+  - rewrite H0.
+    eapply ctxmap_erase_poLe_single. eauto.
+  - rewrite H0. rewrite ctxmap_erase_poEq. reflexivity.
+    eapply x_in_range. split. omega. omega.
+Qed.
+
+Lemma ctxmap_extend_poEq X `{PartialOrder X} n m m'
+  : m ≣ m'
+    -> ctxmap_extend m n ≣ ctxmap_extend m' n.
+Proof.
+  intros. destruct H0.
+  unfold ctxmap_extend; hnf. simpl.
+  split; eauto. intros.
+  decide (x < ctxmap_len m).
+  - rewrite H0.
+    eapply ctxmap_erase_poEq_single. eauto.
+  - rewrite H0. rewrite ctxmap_erase_poEq. reflexivity.
+    eapply x_in_range. split. omega. omega.
+Qed.
+
+Hint Resolve ctxmap_extend_poLe ctxmap_extend_poEq.
